proof/rejection_sampling/UniformSampling_Concrete.ec
@@ -480,6 +480,16 @@ qed.
 
 require import UniformSampling_Abstract.
 
+import RSP.
+lemma jrsample_spec &m a y: 0 <= W64xN.valR y < W64xN.valR a
+  => Pr[ M.rsample(a)@&m: res.`2 = y ] 
+     = Pr[ RSM.RS.sample(fun x => x < W64xN.valR a,0)@&m: res.`2 = W64xN.valR y ].
+  have ->: Pr[ M.rsample(a)@&m: res.`2 = y ] = Pr[CSpecFp.rsample(W64xN.valR a) @ &m : res.`2 = W64xN.valR y ].
+  byequiv. conseq rsample_cspec. smt(). smt(@W64xN). auto. auto.
+move => interval.
+apply (rsample_pr2 (W64xN.valR a) &m (fun (x : int * int) => x.`2 = (W64xN.valR y))).
+qed.
+
 equiv rsample_aspec:
  M.rsample ~ ASpecFp.rsample:
   W64xN.valR byte_z{1} = a{2} /\ 0 < a{2}
@@ -502,6 +512,16 @@ conseq (rsample_eq P  ).
 progress.
 qed.
 
+
+lemma jrsample_pmf &m a y: 0 <= W64xN.valR y < W64xN.valR a
+  => Pr[ M.rsample(a)@&m: res.`2 = y ] = 1%r/(W64xN.valR a)%r.
+proof. move => interval.
+  have ->: 1%r/(W64xN.valR a)%r = Pr[CSpecFp.rsample(W64xN.valR a) @ &m : res.`2 = W64xN.valR y ].
+  rewrite - (rsample_uni &m (W64xN.valR y) (W64xN.valR a)).
+  smt(@W64xN).   smt(@W64xN). smt(). auto.
+byequiv. conseq rsample_cspec. smt(). 
+progress. smt(@W64xN). smt(@W64xN).  auto. auto.
+qed.
 
 (* equiv usample_aspec: *)
 (*  M.usample ~ ASpecFp.rsample: *)
